use a better ghost state theory for value_sensitivity_3

theories/examples/value_sensitivity_3.v
@@ -60,7 +60,30 @@ Definition intermediate := Excl' Intermediate.
 Definition declassified := Excl' Declassified.
 
 Section ghost_state.
-  Context `{!stateG Σ}.
+  Context `{!stateG Σ, !oneshotG Σ}.
+
+  (* Preorder on states *)
+  Definition state_leq (s1 s2 : state) :=
+    match s1, s2 with
+    | Classified,   _            => true
+    | _,            Declassified => true
+    | Intermediate, Intermediate => true
+    | _,            _            => false
+    end.
+
+  Definition in_state γ (s : state) :=
+    match s with
+    | Classified   => own γ.1 (● classified)   ∗ pending γ.2
+    | Intermediate => own γ.1 (● intermediate) ∗ pending γ.2
+    | Declassifed  => own γ.1 (● declassified) ∗ shot γ.2
+    end%I.
+
+  Definition state_token γ (s : state) :=
+    match s with
+    | Classified   => own γ.1 (◯ classified)
+    | Intermediate => own γ.1 (◯ intermediate)
+    | Declassifed  => shot γ.2
+    end%I.
 
   (* TODO: move *)
   Lemma Some_None_not_included {A : cmraT} (x : A) :
@@ -70,6 +93,7 @@ Section ghost_state.
     destruct Hfoo as [a [b [? [? ?]]]]. simplify_eq/=.
   Qed.
 
+  (* Helper lemmas *)
   Lemma current_state γ s1 s2 :
     own γ (◯ Some s2) -∗ own γ (● Some s1) -∗ ⌜s1 = s2⌝.
   Proof.
@@ -82,13 +106,53 @@ Section ghost_state.
     + exfalso. eapply (exclusive_included _ _ Hfoo). done.
   Qed.
 
-  Lemma change_state s2 s1 γ :
+  Lemma excl_change_state s2 s1 γ :
     own γ (● Excl' s1) -∗ own γ (◯ Excl' s1) ==∗ own γ (● Excl' s2) ∗ own γ (◯ Excl' s2).
   Proof.
     apply bi.wand_intro_r. rewrite - !own_op.
     apply own_update. apply auth_update.
     apply option_local_update.
     apply exclusive_local_update. done.
+  Qed.
+
+  (** Ghost state theorey *)
+  Lemma in_state_agree γ s1 s2 :
+    in_state γ s1 -∗ state_token γ s2 -∗ ⌜s1 = s2⌝.
+  Proof.
+    rewrite /in_state /state_token.
+    destruct s1, s2; first
+       [ by iIntros "? ?"; iPureIntro; eauto
+       | iIntros "[Ha _] Hf"; iExFalso;
+         iDestruct (current_state with "Hf Ha") as %Hfoo;
+         simplify_eq/=
+       | iIntros "[_ H1] H2"; iExFalso;
+         iApply (shot_not_pending with "H2 H1") ].
+  Qed.
+
+  Lemma declassified_get_token γ :
+    in_state γ Declassified -∗ in_state γ Declassified ∗ state_token γ Declassified.
+  Proof. simpl. iIntros "[$ #$]". Qed.
+
+  Global Instance declassified_token_persistent γ :
+    Persistent (state_token γ Declassified).
+  Proof. apply _. Qed.
+
+  Lemma state_change γ s2 s3 :
+    state_leq s2 s3 →
+    in_state γ s2 -∗ state_token γ s2 ==∗ in_state γ s3 ∗ state_token γ s3.
+  Proof.
+    rewrite /in_state /state_token. iIntros (Hleq).
+    destruct s2, s3; first
+      [ by iIntros "[$ $] $"
+      | iIntros "[Ha $] Hf"; iApply (excl_change_state with "Ha Hf")
+      | exfalso; by simplify_eq/=
+      | idtac ].
+    - iIntros "[Ha H] Hf".
+      iMod (shoot with "H") as "#$".
+      by iMod (excl_change_state with "Ha Hf") as "[$ _]".
+    - iIntros "[Ha H] Hf".
+      iMod (shoot with "H") as "#$".
+      by iMod (excl_change_state with "Ha Hf") as "[$ _]".
   Qed.
 
 End ghost_state.
@@ -99,13 +163,13 @@ Section proof.
   (* The invariant guarantees the monotonicity of the declassification. *)
   Definition inv_body (r1 r2 : rec) γ γs ξ :=
     (* in the state CLASSIFIED *)
-    ((∃ v1 v2, own γ (● classified) ∗ pending γs ∗ r1.1 ↦ₗ #true ∗ r2.1 ↦ᵣ #true
+    ((∃ v1 v2, in_state (γ, γs) Classified ∗ r1.1 ↦ₗ #true ∗ r2.1 ↦ᵣ #true
                    ∗ r1.2 ↦ₗ v1 ∗ r2.2 ↦ᵣ v2 ∗ ⟦ tint High ⟧ ξ v1 v2)
    ∨ (* in the state INTERMEDIATE *)
-     (∃ v, own γ (● intermediate) ∗ pending γs ∗ r1.1 ↦ₗ #true ∗ r2.1 ↦ #true
+     (∃ v, in_state (γ, γs) Intermediate ∗ r1.1 ↦ₗ #true ∗ r2.1 ↦ #true
                ∗ r1.2 ↦ₗ v ∗ r2.2 ↦ᵣ v ∗ ⟦ tint Low ⟧ ξ v v)
    ∨ (* in the state DECLASSIFIED *)
-     (∃ v, own γ (● declassified) ∗ shot γs ∗ r1.1 ↦ₗ #false ∗ r2.1 ↦ #false
+     (∃ v, in_state (γ, γs) Declassified ∗ r1.1 ↦ₗ #false ∗ r2.1 ↦ #false
                ∗ r1.2 ↦ₗ v ∗ r2.2 ↦ᵣ v ∗ ⟦ tint Low ⟧ ξ v v))%I.
 
   Definition N := nroot.@"example".
@@ -126,19 +190,20 @@ Section proof.
     iApply dwp_atomic.
     iInv N as "[Hst|[Hst|Hst]]" "Hcl"; iModIntro.
     - (* We are still in the CLASSIFIED state *)
-      iDestruct "Hst" as (v1 v2) "(Hstate & Htok & Hi1 & Hi2 & Hd1 & Hd2 & Hv)".
+      iDestruct "Hst" as (v1 v2) "(Hstate & Hi1 & Hi2 & Hd1 & Hd2 & Hv)".
       iApply (dwp_load with "Hi1 Hi2"). iIntros "Hi1 Hi2". iNext.
       iMod ("Hcl" with "[-]") as "_".
       { iNext. iLeft. eauto with iFrame. }
       iModIntro. dwp_pures. by iApply "IH".
     - (* We are in the INTERMEDIATE state *)
-      iDestruct "Hst" as (v) "(Hstate & Htok & Hi1 & Hi2 & Hd1 & Hd2 & Hv)".
+      iDestruct "Hst" as (v) "(Hstate & Hi1 & Hi2 & Hd1 & Hd2 & Hv)".
       iApply (dwp_load with "Hi1 Hi2"). iIntros "Hi1 Hi2". iNext.
       iMod ("Hcl" with "[-]") as "_".
       { iNext. iRight. iLeft. eauto with iFrame. }
       iModIntro. dwp_pures. by iApply "IH".
     - (* We are in the DECLASSIFIED state *)
-      iDestruct "Hst" as (v) "(Hstate & #Hdecl & Hi1 & Hi2 & Hd1 & Hd2 & Hv)".
+      iDestruct "Hst" as (v) "(Hstate & Hi1 & Hi2 & Hd1 & Hd2 & Hv)".
+      iMod (declassified_get_token with "Hstate") as "[Hstate #Hdecl]".
       iApply (dwp_load with "Hi1 Hi2"). iIntros "Hi1 Hi2". iNext.
       iMod ("Hcl" with "[-]") as "_".
       { iNext. iRight. iRight. eauto with iFrame. }
@@ -151,17 +216,15 @@ Section proof.
       iApply dwp_atomic.
       iInv N as "[Hst|[Hst|Hst]]" "Hcl"; iModIntro.
       + (* We *cannot* be in the CLASSIFIED state *)
-        iDestruct "Hst" as (v1 v2) "(Hstate & >Htok & Hi1 & Hi2 & Hd1 & Hd2 & Hv)".
-        iExFalso. iApply (shot_not_pending with "Hdecl Htok").
-      + (* We also cannot be in the INTERMEDIATE state, but we do not
-           really care about that here. *)
-        iDestruct "Hst" as (v) "(Hstate & Htok & Hi1 & Hi2 & Hd1 & Hd2 & #Hv)".
-        iApply (dwp_load with "Hd1 Hd2"). iIntros "Hd1 Hd2". iNext.
-        iMod ("Hcl" with "[-]") as "_".
-        { iNext. iRight. iLeft. eauto with iFrame. }
-        iModIntro. iApply logrel_store; first solve_ndisj; by iApply dwp_value.
+        iDestruct "Hst" as (v1 v2) "(>Hstate & Hi1 & Hi2 & Hd1 & Hd2 & Hv)".
+        iExFalso. iDestruct (in_state_agree with "Hstate Hdecl") as %foo.
+        simplify_eq/=.
+      + (* We *cannot* be in the INTERMEDIATE state *)
+        iDestruct "Hst" as (v) "(>Hstate & Hi1 & Hi2 & Hd1 & Hd2 & #Hv)".
+        iExFalso. iDestruct (in_state_agree with "Hstate Hdecl") as %foo.
+        simplify_eq/=.
       + (* Still in the DECLASSIFIED state *)
-        iDestruct "Hst" as (v) "(Hstate & Hfrag & Hi1 & Hi2 & Hd1 & Hd2 & #Hv)".
+        iDestruct "Hst" as (v) "(Hstate & Hi1 & Hi2 & Hd1 & Hd2 & #Hv)".
         iApply (dwp_load with "Hd1 Hd2"). iIntros "Hd1 Hd2". iNext.
         iMod ("Hcl" with "[-]") as "_".
         { iNext. iRight. iRight. eauto with iFrame. }
@@ -170,7 +233,7 @@ Section proof.
 
   Lemma thread2_spec γ rec1 rec2 ξ :
     I rec1 rec2 γ ξ -∗
-    own γ.1 (◯ classified) -∗
+    state_token γ Classified -∗
     DWP thread2 rec1 & thread2 rec2 : ⟦ tunit ⟧ ξ.
   Proof.
     iDestruct 1 as (ri1 ri2 rd1 rd2 -> ->) "#Hinv".
@@ -180,36 +243,45 @@ Section proof.
     iApply dwp_atomic.
     iInv N as "[Hst|[Hst|Hst]]" "Hcl"; iModIntro.
     - (* We are still in the CLASSIFIED state *)
-      iDestruct "Hst" as (v1 v2) "(Hstate & Htok & Hi1 & Hi2 & Hd1 & Hd2 & Hv)".
+      iDestruct "Hst" as (v1 v2) "(Hstate & Hi1 & Hi2 & Hd1 & Hd2 & Hv)".
       iApply (dwp_store with "Hd1 Hd2"). iIntros "Hd1 Hd2". iNext.
-      iMod (change_state Intermediate with "Hstate Hstt") as "[Hstate Hstt]".
+      iMod (state_change _ _ Intermediate with "Hstate Hstt") as "[Hstate Hstt]";
+        first done.
       iMod ("Hcl" with "[-Hstt]") as "_".
       { iNext. iRight. iLeft. iExists #0. iFrame.
         rewrite interp_eq. iExists 0,0. eauto with iFrame. } clear v1 v2.
       iModIntro. dwp_pures. iApply dwp_atomic.
       iInv N as "[Hst|[Hst|Hst]]" "Hcl"; iModIntro.
       + (* CLASSIFIED state --> impossible *)
-        iDestruct "Hst" as (v1 v2) "(>Hstate & Htok & Hi1 & Hi2 & Hd1 & Hd2 & Hv)".
-        iDestruct (current_state with "Hstt Hstate") as %Hfoo.
-        simplify_eq/=.
+        iDestruct "Hst" as (v1 v2) "(>Hstate & Hi1 & Hi2 & Hd1 & Hd2 & Hv)".
+        iDestruct (in_state_agree with "Hstate Hstt") as %Hfoo.
+        exfalso. naive_solver.
       + (* INTERMEDIATE state *)
-        iDestruct "Hst" as (v) "(Hstate & Htok & Hi1 & Hi2 & Hd1 & Hd2 & Hv)".
+        iDestruct "Hst" as (v) "(Hstate & Hi1 & Hi2 & Hd1 & Hd2 & Hv)".
         iApply (dwp_store with "Hi1 Hi2"). iIntros "Hi1 Hi2". iNext.
-        iMod (change_state Declassified with "Hstate Hstt") as "[Hstate Hstt]".
-        iMod (shoot with "Htok") as "Htok".
+        iMod (state_change _ _ Declassified with "Hstate Hstt") as "[Hstate Hstt]";
+          first done.
         iMod ("Hcl" with "[-Hstt]") as "_".
         { iNext. iRight. iRight. eauto with iFrame.  }
         iModIntro. eauto with iFrame.
-      + (* DECLASSIFIED state --> impossible *)
-        iDestruct "Hst" as (v) "(>Hstate & Htok & Hi1 & Hi2 & Hd1 & Hd2 & Hv)".
-        iDestruct (current_state with "Hstt Hstate") as %Hfoo.
-        simplify_eq/=.
+      + (* DECLASSIFIED state. In this case it is actually impossible
+           in the program, but we don't account for that in the proof.
+           Instead we can just keep calm and carry on. *)
+        iDestruct "Hst" as (v) "(>Hstate & Hi1 & Hi2 & Hd1 & Hd2 & Hv)".
+        iApply (dwp_store with "Hi1 Hi2"). iIntros "Hi1 Hi2". iNext.
+        iMod ("Hcl" with "[-Hstt]") as "_".
+        { iNext. iRight. iRight. eauto with iFrame.  }
+        iModIntro. eauto with iFrame.
     - (* INTERMEDIATE state --> impossible *)
-      iDestruct "Hst" as (v) "(>Hstate & Htok & Hi1 & Hi2 & Hd1 & Hd2 & Hv)".
-      iDestruct (current_state with "Hstt Hstate") as %Hfoo. simplify_eq/=.
+      iDestruct "Hst" as (v) "(>Hstate & Hi1 & Hi2 & Hd1 & Hd2 & Hv)".
+      destruct γ as [γ γs].
+      iDestruct (in_state_agree with "Hstate Hstt") as %Hfoo.
+      exfalso. naive_solver.
     - (* DECLASSIFIED state --> impossible *)
-      iDestruct "Hst" as (v) "(>Hstate & Htok & Hi1 & Hi2 & Hd1 & Hd2 & Hv)".
-      iDestruct (current_state with "Hstt Hstate") as %Hfoo. simplify_eq/=.
+      iDestruct "Hst" as (v) "(>Hstate & Hi1 & Hi2 & Hd1 & Hd2 & Hv)".
+      destruct γ as [γ γs].
+      iDestruct (in_state_agree with "Hstate Hstt") as %Hfoo.
+      exfalso. naive_solver.
   Qed.
 
 
